proof/theories/Optiplex_Gen.v
@@ -12,18 +12,25 @@ Open Scope string_scope.
 Definition decls : set_decls :=
   {| sd_sets := [("vmaddrs", [([192; 168; 51; 20], [192; 168; 51; 20]); ([192; 168; 51; 14], [192; 168; 51; 14]); ([192; 168; 51; 15], [192; 168; 51; 15]); ([192; 168; 51; 12], [192; 168; 51; 12]); ([192; 168; 51; 10], [192; 168; 51; 10]); ([192; 168; 51; 1], [192; 168; 51; 1]); ([192; 168; 51; 21], [192; 168; 51; 21]); ([192; 168; 51; 22], [192; 168; 51; 22]); ([192; 168; 51; 23], [192; 168; 51; 23]); ([192; 168; 51; 24], [192; 168; 51; 24])]);
    ("vmantispoof", [([192; 168; 51; 20; 105; 110; 99; 45; 98; 117; 100; 103; 101], [192; 168; 51; 20; 105; 110; 99; 45; 98; 117; 100; 103; 101]); ([192; 168; 51; 14; 105; 110; 99; 45; 118; 105; 107; 117; 110], [192; 168; 51; 14; 105; 110; 99; 45; 118; 105; 107; 117; 110]); ([192; 168; 51; 15; 105; 110; 99; 45; 102; 114; 101; 115; 104], [192; 168; 51; 15; 105; 110; 99; 45; 102; 114; 101; 115; 104]); ([192; 168; 51; 12; 118; 98; 45; 103; 101; 110; 116; 111; 111], [192; 168; 51; 12; 118; 98; 45; 103; 101; 110; 116; 111; 111]); ([192; 168; 51; 10; 118; 98; 45; 104; 97; 115; 115], [192; 168; 51; 10; 118; 98; 45; 104; 97; 115; 115]); ([192; 168; 51; 1; 118; 108; 97; 110; 46; 50; 48], [192; 168; 51; 1; 118; 108; 97; 110; 46; 50; 48]); ([192; 168; 51; 21; 118; 98; 45; 109; 101; 109; 111; 115], [192; 168; 51; 21; 118; 98; 45; 109; 101; 109; 111; 115]); ([192; 168; 51; 22; 118; 98; 45; 105; 115; 115; 111], [192; 168; 51; 22; 118; 98; 45; 105; 115; 115; 111]); ([192; 168; 51; 23; 118; 98; 45; 110; 116; 102; 121], [192; 168; 51; 23; 118; 98; 45; 110; 116; 102; 121]); ([192; 168; 51; 24; 118; 98; 45; 99; 111; 108; 108], [192; 168; 51; 24; 118; 98; 45; 99; 111; 108; 108])]);
-   ("__set0", [([0; 0; 0; 2], [0; 0; 0; 2]); ([0; 0; 0; 4], [0; 0; 0; 4])]);
+   ("__set0", [([6], [6]); ([17], [17])]);
    ("__set1", [([108; 97; 110; 48], [108; 97; 110; 48]); ([104; 111; 109; 101], [104; 111; 109; 101])]);
-   ("__set2", [([0; 22], [0; 22]); ([0; 80], [0; 80]); ([1; 187], [1; 187]); ([4; 222], [4; 222])]);
-   ("__set3", [([108; 97; 110; 48], [108; 97; 110; 48]); ([104; 111; 109; 101], [104; 111; 109; 101])]);
-   ("__set4", [([6], [6]); ([17], [17])]);
-   ("__set5", [([116; 115], [116; 118]); ([105; 137], [105; 137]); ([106; 81], [106; 81]); ([31; 107], [31; 107])]);
-   ("__set6", [([6], [6]); ([17], [17])]);
+   ("__set2", [([6], [6]); ([17], [17])]);
+   ("__set3", [([187; 112], [187; 112]); ([187; 117], [187; 117]); ([187; 138], [187; 138]); ([187; 126], [187; 126]); ([187; 127], [187; 127]); ([187; 128], [187; 128]); ([187; 130], [187; 130])]);
+   ("__set4", [([108; 97; 110; 48], [108; 97; 110; 48]); ([104; 111; 109; 101], [104; 111; 109; 101])]);
+   ("__set5", [([6], [6]); ([17], [17])]);
+   ("__set6", [([187; 112], [187; 112]); ([187; 117], [187; 117]); ([187; 138], [187; 138]); ([187; 126], [187; 126]); ([187; 127], [187; 127]); ([187; 128], [187; 128]); ([187; 130], [187; 130])]);
    ("__set7", [([0; 0; 0; 2], [0; 0; 0; 2]); ([0; 0; 0; 4], [0; 0; 0; 4])]);
-   ("__set8", [([0; 0; 0; 153], [0; 0; 0; 153]); ([0; 0; 1; 0], [0; 0; 1; 0])]);
-   ("__set9", [([118; 98; 45; 106; 101; 108; 108; 121; 115; 101; 101; 114; 114], [118; 98; 45; 106; 101; 108; 108; 121; 115; 101; 101; 114; 114]); ([118; 98; 45; 115; 97; 98; 110; 122; 98; 100], [118; 98; 45; 115; 97; 98; 110; 122; 98; 100]); ([118; 98; 45; 114; 97; 100; 97; 114], [118; 98; 45; 114; 97; 100; 97; 114])]);
-   ("__set10", [([118; 98; 45; 106; 101; 108; 108; 121; 115; 101; 101; 114; 114], [118; 98; 45; 106; 101; 108; 108; 121; 115; 101; 101; 114; 114]); ([118; 98; 45; 115; 97; 98; 110; 122; 98; 100], [118; 98; 45; 115; 97; 98; 110; 122; 98; 100]); ([118; 98; 45; 114; 97; 100; 97; 114], [118; 98; 45; 114; 97; 100; 97; 114])]);
-   ("__set11", [([0; 0; 0; 2], [0; 0; 0; 2]); ([0; 0; 0; 4], [0; 0; 0; 4])])];
+   ("__set8", [([108; 97; 110; 48], [108; 97; 110; 48]); ([104; 111; 109; 101], [104; 111; 109; 101])]);
+   ("__set9", [([0; 22], [0; 22]); ([0; 80], [0; 80]); ([1; 187], [1; 187]); ([4; 222], [4; 222])]);
+   ("__set10", [([108; 97; 110; 48], [108; 97; 110; 48]); ([104; 111; 109; 101], [104; 111; 109; 101])]);
+   ("__set11", [([6], [6]); ([17], [17])]);
+   ("__set12", [([116; 115], [116; 118]); ([105; 137], [105; 137]); ([106; 81], [106; 81]); ([31; 107], [31; 107])]);
+   ("__set13", [([6], [6]); ([17], [17])]);
+   ("__set14", [([0; 0; 0; 2], [0; 0; 0; 2]); ([0; 0; 0; 4], [0; 0; 0; 4])]);
+   ("__set15", [([0; 0; 0; 153], [0; 0; 0; 153]); ([0; 0; 1; 0], [0; 0; 1; 0])]);
+   ("__set16", [([118; 98; 45; 106; 101; 108; 108; 121; 115; 101; 101; 114; 114], [118; 98; 45; 106; 101; 108; 108; 121; 115; 101; 101; 114; 114]); ([118; 98; 45; 115; 97; 98; 110; 122; 98; 100], [118; 98; 45; 115; 97; 98; 110; 122; 98; 100]); ([118; 98; 45; 114; 97; 100; 97; 114], [118; 98; 45; 114; 97; 100; 97; 114])]);
+   ("__set17", [([118; 98; 45; 106; 101; 108; 108; 121; 115; 101; 101; 114; 114], [118; 98; 45; 106; 101; 108; 108; 121; 115; 101; 101; 114; 114]); ([118; 98; 45; 115; 97; 98; 110; 122; 98; 100], [118; 98; 45; 115; 97; 98; 110; 122; 98; 100]); ([118; 98; 45; 114; 97; 100; 97; 114], [118; 98; 45; 114; 97; 100; 97; 114])]);
+   ("__set18", [([0; 0; 0; 2], [0; 0; 0; 2]); ([0; 0; 0; 4], [0; 0; 0; 4])])];
    sd_vmaps := [];
    sd_maps := [] |}.
 
@@ -38,7 +45,32 @@ Definition gen_env : env := env_with_sets base_env decls.
 
 Definition filter_prerouting : chain :=
   {| c_policy := Accept;
-   c_rules := [] |}.
+   c_rules := [{| r_body := [(BMatch (MEq FMetaIifname [104; 111; 109; 101]));
+             (BMatch (MEq (FFib "daddr" FRtype) [0; 0; 0; 2]));
+             (BMatch (MConcatSet [FMetaL4proto] false "__set0"));
+             (BMatch (MEq FThDport [13; 61]));
+             (BStmt (SMetaSet MKmark (VImm [0; 0; 0; 153])));
+             (BStmt (SLog "[nft:rdppre]"))];
+     r_verdict := Accept; r_vmap := None;
+     r_nat := None; r_tproxy := None; r_fwd := None; r_queue := None; r_after := [] |};
+
+   {| r_body := [(BMatch (MConcatSet [FMetaIifname] false "__set1"));
+             (BMatch (MEq (FFib "daddr" FRtype) [0; 0; 0; 2]));
+             (BMatch (MConcatSet [FMetaL4proto] false "__set2"));
+             (BMatch (MConcatSet [FThDport] false "__set3"));
+             (BStmt (SMetaSet MKmark (VImm [0; 0; 0; 153])));
+             (BStmt (SLog "[nft:rdppre]"))];
+     r_verdict := Accept; r_vmap := None;
+     r_nat := None; r_tproxy := None; r_fwd := None; r_queue := None; r_after := [] |};
+
+   {| r_body := [(BMatch (MConcatSet [FMetaIifname] false "__set4"));
+             (BMatch (MEq (FFib "daddr" FRtype) [0; 0; 0; 2]));
+             (BMatch (MConcatSet [FMetaL4proto] false "__set5"));
+             (BMatch (MConcatSet [FThDport] false "__set6"));
+             (BStmt (SMetaSet MKmark (VImm [0; 0; 0; 153])));
+             (BStmt (SLog "[nft:rdppre]"))];
+     r_verdict := Accept; r_vmap := None;
+     r_nat := None; r_tproxy := None; r_fwd := None; r_queue := None; r_after := [] |}] |}.
 
 Definition filter_postrouting : chain :=
   {| c_policy := Accept;
@@ -49,7 +81,7 @@ Definition filter_postrouting : chain :=
 
 Definition filter_input : chain :=
   {| c_policy := Drop;
-   c_rules := [{| r_body := [(BMatch (MConcatSet [FCtState] false "__set0"))];
+   c_rules := [{| r_body := [(BMatch (MConcatSet [FCtState] false "__set7"))];
      r_verdict := Accept; r_vmap := None;
      r_nat := None; r_tproxy := None; r_fwd := None; r_queue := None; r_after := [] |};
 
@@ -90,21 +122,21 @@ Definition filter_input : chain :=
      r_verdict := Accept; r_vmap := None;
      r_nat := None; r_tproxy := None; r_fwd := None; r_queue := None; r_after := [] |};
 
-   {| r_body := [(BMatch (MConcatSet [FMetaIifname] false "__set1"));
+   {| r_body := [(BMatch (MConcatSet [FMetaIifname] false "__set8"));
              (BMatch (MEq FMetaL4proto [6]));
-             (BMatch (MConcatSet [FThDport] false "__set2"))];
+             (BMatch (MConcatSet [FThDport] false "__set9"))];
      r_verdict := Accept; r_vmap := None;
      r_nat := None; r_tproxy := None; r_fwd := None; r_queue := None; r_after := [] |};
 
-   {| r_body := [(BMatch (MConcatSet [FMetaIifname] false "__set3"));
-             (BMatch (MConcatSet [FMetaL4proto] false "__set4"));
+   {| r_body := [(BMatch (MConcatSet [FMetaIifname] false "__set10"));
+             (BMatch (MConcatSet [FMetaL4proto] false "__set11"));
              (BMatch (MEq FThDport [85; 240]))];
      r_verdict := Accept; r_vmap := None;
      r_nat := None; r_tproxy := None; r_fwd := None; r_queue := None; r_after := [] |};
 
    {| r_body := [(BMatch (MEq FMetaIifname [108; 97; 110; 48]));
              (BMatch (MEq FMetaL4proto [6]));
-             (BMatch (MConcatSet [FThDport] false "__set5"))];
+             (BMatch (MConcatSet [FThDport] false "__set12"))];
      r_verdict := Accept; r_vmap := None;
      r_nat := None; r_tproxy := None; r_fwd := None; r_queue := None; r_after := [] |};
 
@@ -122,7 +154,7 @@ Definition filter_input : chain :=
      r_nat := None; r_tproxy := None; r_fwd := None; r_queue := None; r_after := [] |};
 
    {| r_body := [(BMatch (MEq FMetaIifname [105; 109; 109; 105; 99; 104]));
-             (BMatch (MConcatSet [FMetaL4proto] false "__set6"));
+             (BMatch (MConcatSet [FMetaL4proto] false "__set13"));
              (BMatch (MEq FThDport [0; 53]))];
      r_verdict := Accept; r_vmap := None;
      r_nat := None; r_tproxy := None; r_fwd := None; r_queue := None; r_after := [] |};
@@ -152,11 +184,11 @@ Definition filter_forward : chain :=
      r_verdict := Accept; r_vmap := None;
      r_nat := None; r_tproxy := None; r_fwd := None; r_queue := None; r_after := [] |};
 
-   {| r_body := [(BMatch (MConcatSet [FCtState] false "__set7"))];
+   {| r_body := [(BMatch (MConcatSet [FCtState] false "__set14"))];
      r_verdict := Accept; r_vmap := None;
      r_nat := None; r_tproxy := None; r_fwd := None; r_queue := None; r_after := [] |};
 
-   {| r_body := [(BMatch (MConcatSet [FMetaMark] false "__set8"));
+   {| r_body := [(BMatch (MConcatSet [FMetaMark] false "__set15"));
              (BStmt (SLog "[nft:rdpforward]"))];
      r_verdict := Accept; r_vmap := None;
      r_nat := None; r_tproxy := None; r_fwd := None; r_queue := None; r_after := [] |}] |}.
@@ -181,8 +213,8 @@ Definition vmfilter_vm : chain :=
      r_verdict := Accept; r_vmap := None;
      r_nat := None; r_tproxy := None; r_fwd := None; r_queue := None; r_after := [] |};
 
-   {| r_body := [(BMatch (MConcatSet [FMetaIifname] false "__set9"));
-             (BMatch (MConcatSet [FMetaOifname] false "__set10"))];
+   {| r_body := [(BMatch (MConcatSet [FMetaIifname] false "__set16"));
+             (BMatch (MConcatSet [FMetaOifname] false "__set17"))];
      r_verdict := Accept; r_vmap := None;
      r_nat := None; r_tproxy := None; r_fwd := None; r_queue := None; r_after := [] |}] |}.
 
@@ -224,7 +256,7 @@ Definition vmfilter_forward : chain :=
      r_verdict := Accept; r_vmap := None;
      r_nat := None; r_tproxy := None; r_fwd := None; r_queue := None; r_after := [] |};
 
-   {| r_body := [(BMatch (MConcatSet [FCtState] false "__set11"))];
+   {| r_body := [(BMatch (MConcatSet [FCtState] false "__set18"))];
      r_verdict := Accept; r_vmap := None;
      r_nat := None; r_tproxy := None; r_fwd := None; r_queue := None; r_after := [] |};
 
